Add source to chain traces
Instead of traces always starting from the empty environment and an
empty queue, they can now start from any environment and queue. This
should hopefully make it simpler for us to define what it means to be a
prefix of a trace.

src/Blockchain.v
@@ -410,7 +410,7 @@ Record Environment :=
 (* Furthermore we define extensional equality for such environments. *)
 Record EnvironmentEquiv (e1 e2 : Environment) : Prop :=
   build_env_equiv {
-    chain_equiv :> ChainEquiv e1 e2;
+    chain_equiv : ChainEquiv e1 e2;
     contracts_eq : forall a, env_contracts e1 a = env_contracts e2 a;
   }.
 
@@ -614,7 +614,7 @@ Proof.
   unfold account_balance.
   destruct step;
     match goal with
-    | [H: EnvironmentEquiv _ _ |- _] => rewrite (H : ChainEquiv _ _)
+    | [H: EnvironmentEquiv _ _ |- _] => rewrite H
     end;
     simpl; unfold add_tx_to_map; destruct_address_eq; simpl; lia.
 Qed.
@@ -655,6 +655,17 @@ Proof.
 Qed.
 End Step.
 
+Lemma chain_step_respects_equiv e1 e2 act tx e1' e2' new_acts :
+  EnvironmentEquiv e1 e2 ->
+  EnvironmentEquiv e1' e2' ->
+  ChainStep e1 act tx e1' new_acts ->
+  ChainStep e2 act tx e2' new_acts.
+Proof.
+  Hint Constructors ChainStep : core.
+  intros eq eq' step.
+  destruct step; rewrite eq, eq' in *; eauto.
+Qed.
+
 Definition add_new_block_header
           (header : BlockHeader)
           (baker : Address)
@@ -679,7 +690,7 @@ Definition IsValidNextBlock (new old : BlockHeader) : Prop :=
   finalized_height new >= finalized_height old /\
   finalized_height new < block_height new.
 
-Definition initial_env :=
+Definition empty_env : Environment :=
   {| env_chain :=
        {| block_header :=
             {| block_height := 0;
@@ -691,71 +702,72 @@ Definition initial_env :=
           contract_state a := None; |};
      env_contracts a := None; |}.
 
-(* The chain captures that an environment can be reached
-with some current actions queued. *)
-Inductive ChainTrace : Environment -> list Action -> Prop :=
-  | ctrace_initial :
-      forall (env : Environment),
-        EnvironmentEquiv env initial_env ->
-        ChainTrace env []
+(* The ChainTrace captures there is a valid execution where, starting
+from one environment and queue of actions, we end up in a different
+environment and queue of actions. *)
+Inductive ChainTrace :
+  Environment -> list Action ->
+  Environment -> list Action -> Prop :=
+  | ctrace_refl :
+      forall (env env' : Environment) (l : list Action),
+        EnvironmentEquiv env env' ->
+        ChainTrace env l env' l
   (* Add a new block to the trace *)
   | ctrace_block :
-      forall (prev : Environment)
+      forall (from : Environment)
+             (from_queue : list Action)
+             (prev_to : Environment)
              (header : BlockHeader)
              (baker : Address)
-             (acts : list Action)
-             (new : Environment),
-        ChainTrace prev [] ->
-        IsValidNextBlock header (block_header prev) ->
-        Forall (fun act => address_is_contract (act_from act) = false) acts ->
+             (to : Environment)
+             (queue : list Action),
+        ChainTrace from from_queue prev_to [] ->
+        IsValidNextBlock header (block_header prev_to) ->
+        Forall (fun act => address_is_contract (act_from act) = false) queue ->
         EnvironmentEquiv
-          new
-          (add_new_block_header header baker prev) ->
-        ChainTrace new acts
+          to
+          (add_new_block_header header baker prev_to) ->
+        ChainTrace from from_queue to queue
   (* Execute an action *)
   | ctrace_step :
-      forall (prev : Environment)
+      forall (from : Environment)
+             (from_queue : list Action)
+             (prev_to : Environment)
              (act : Action)
              (acts : list Action)
              (tx : Tx)
              (new : Environment)
              (new_acts : list Action),
-        ChainTrace prev (act :: acts) ->
-        ChainStep prev act tx new new_acts ->
-        ChainTrace new (new_acts ++ acts)
+        ChainTrace from from_queue prev_to (act :: acts) ->
+        ChainStep prev_to act tx new new_acts ->
+        ChainTrace from from_queue new (new_acts ++ acts)
   (* Reorder action order *)
   | ctrace_permute :
-      forall (env : Environment)
-             (acts acts' : list Action),
-        ChainTrace env acts ->
-        Permutation acts acts' ->
-        ChainTrace env acts'.
+      forall (from : Environment)
+             (from_queue : list Action)
+             (to : Environment)
+             (to_queue to_queue' : list Action),
+        ChainTrace from from_queue to to_queue ->
+        Permutation to_queue to_queue' ->
+        ChainTrace from from_queue to to_queue'.
 
-Lemma chain_step_respects_equiv e1 e2 act tx e1' e2' new_acts :
-  EnvironmentEquiv e1 e2 ->
-  EnvironmentEquiv e1' e2' ->
-  ChainStep e1 act tx e1' new_acts ->
-  ChainStep e2 act tx e2' new_acts.
+Lemma chain_trace_respects_equiv from from' to to' from_queue to_queue :
+  EnvironmentEquiv from from' ->
+  EnvironmentEquiv to to' ->
+  ChainTrace from from_queue to to_queue ->
+  ChainTrace from' from_queue to' to_queue.
 Proof.
-  Hint Constructors ChainStep : core.
-  intros eq eq' step.
-  destruct step; rewrite eq, eq' in *; eauto.
-Qed.
-
-Lemma chain_trace_respects_equiv e1 e2 l :
-  EnvironmentEquiv e1 e2 ->
-  ChainTrace e1 l ->
-  ChainTrace e2 l.
-Proof.
-  intros eq trace.
-  Hint Resolve ctrace_initial ctrace_block ctrace_step : core.
+  Hint Resolve ctrace_refl ctrace_block ctrace_step : core.
   Hint Resolve chain_step_respects_equiv.
-  Hint Extern 1 (ChainTrace ?env _) =>
+  Hint Extern 1 (ChainTrace _ _ _ _) =>
   match goal with
-  | [H: Permutation ?a ?b |- _] => apply (ctrace_permute env a b)
+  | [H: Permutation ?a ?b |- _] => apply (ctrace_permute _ _ _ a b)
   end.
   Hint Extern 1 (EnvironmentEquiv _ _) => reflexivity.
-  induction trace; eauto; rewrite eq in *; eauto.
+
+  intros eq_from eq_to trace.
+  revert to' eq_to.
+  induction trace; intros to' eq_to; eauto; rewrite eq_from, eq_to in *; eauto.
 Qed.
 End Theories.
 End Semantics.
@@ -777,7 +789,7 @@ Class ChainBuilderType :=
       option builder_type;
 
     builder_trace (b : builder_type) :
-      ChainTrace (builder_env b) [];
+      ChainTrace empty_env [] (builder_env b) [];
   }.
 
 Global Coercion builder_type : ChainBuilderType >-> Sortclass.
